

III

QUANTUM FOURIER TRANSFORM



In classical term Discrete Fourier Transform (DFT), is a map from N complex numbers to N complex numbers (for a vector f):

$$\tilde{f}_j = \frac{1}{\sqrt{N}} \sum_{k=0}^{N-1} \omega^{-jk} f_k. \quad (\text{III.1})$$

where

$$\omega = \exp\left(\frac{2\pi i}{N}\right). \quad (\text{III.2})$$

And, inverse DFT is defined as:

$$f_j = \frac{1}{\sqrt{N}} \sum_{k=0}^{N-1} \omega^{jk} \tilde{f}_k. \quad (\text{III.3})$$

Let $f_k^{(\ell)} = \delta_{k,\ell}$. Then:

$$\tilde{f}_j^{(\ell)} = \frac{1}{\sqrt{N}} \sum_{k=0}^{N-1} \omega^{-jk} \delta_{k,\ell} = \frac{1}{\sqrt{N}} \omega^{-j\ell}. \quad (\text{III.4})$$

ORTHONORMALITY:

$$\sum_j (\tilde{f}_j^{(\ell)})^* \tilde{f}_j^{(m)} = \left(\frac{1}{\sqrt{N}} \right) \left(\frac{1}{\sqrt{N}} \right) \sum_j \omega^{j\ell} \omega^{-jm} \quad (\text{III.5})$$

$$= \frac{1}{N} \sum_j \omega^{j(\ell-m)} = \delta_{\ell m}. \quad (\text{III.6})$$

Another important property is the convolution theorem:

$$(f * g)_k = \sum_{j=0}^{N-1} f_j g_{k-j} \quad (\text{mod } N), \quad (\text{III.7})$$

where (circular convolution) $g_{-m} = g_{N-m}$.

DETOUR: WHAT DOES $k - j$ MEAN? Let's understand it with an example, Assume:

$$f = [1, 2, 3, 4], \quad g = [5, 6, 7, 8].$$

Then

$$(f * g)_0 = f_0 g_{0-0} + f_1 g_{0-1} + f_2 g_{0-2} + f_3 g_{0-3}. \quad (\text{III.8})$$

Using indices modulo $N = 4$:

$$g_0 = 5, \quad g_{0-1} = g_3 = 8, \quad g_{0-2} = g_2 = 7, \quad g_{0-3} = g_1 = 6.$$

So

$$f * g = [(f * g)_0, (f * g)_1, (f * g)_2, (f * g)_3].$$

FAST FOURIER TRANSFORM (FFT) AND APPLICATIONS

For the DFT we need to do N multiplications and then add them, why?

For a vector $x = [x_0, x_1, \dots, x_{N-1}]$, the DFT is defined as

$$\hat{x}_k = \sum_{n=0}^{N-1} x_n e^{-2\pi i k n / N}, \quad k = 0, 1, \dots, N-1. \quad (\text{III.9})$$

So, for each k you compute a sum of N terms:

- N complex multiplications and $\sim (N-1)$ additions,
- total work $\sim N(N-1) \approx N^2$,
- hence $\mathcal{O}(N^2)$ complexity.

FAST FOURIER TRANSFORM (FFT)

Fast Fourier helps make the process faster. Here we assume $N = 2^n$ (the length is a power of 2).

To make the process fast, split the components of f into smaller vectors of size $N/2$:

$$e_i = f_{2i} \quad (\text{even components}), \quad o_i = f_{2i+1} \quad (\text{odd components}).$$

Let $\omega_N = e^{2\pi i / N}$. Then:

$$\tilde{f}_j = \sum_{i=0}^{N-1} f_i \omega_N^{-ij} \quad (\text{III.10})$$

$$= \sum_{i=0}^{N/2-1} f_{2i} \omega_N^{-j(2i)} + \sum_{i=0}^{N/2-1} f_{2i+1} \omega_N^{-j(2i+1)} \quad (\text{III.11})$$

$$= \sum_{i=0}^{N/2-1} e_i \omega_N^{-2ji} + \sum_{i=0}^{N/2-1} o_i \omega_N^{-j} \omega_N^{-2ji}. \quad (\text{III.12})$$

Now, let $\omega_N = e^{2\pi i / N}$ and assume N is even. After splitting

$$e_i := f_{2i} \quad (\text{even part}), \quad o_i := f_{2i+1} \quad (\text{odd part}), \quad i = 0, \dots, \frac{N}{2}-1,$$

the DFT can be written as

$$\tilde{f}_j = \sum_{i=0}^{\frac{N}{2}-1} f_{2i} \omega_N^{-j(2i)} + \sum_{i=0}^{\frac{N}{2}-1} f_{2i+1} \omega_N^{-j(2i+1)} \quad (\text{III.I3})$$

$$= \sum_{i=0}^{\frac{N}{2}-1} e_i \omega_N^{-2ji} + \omega_N^{-j} \sum_{i=0}^{\frac{N}{2}-1} o_i \omega_N^{-2ji}. \quad (\text{III.I4})$$

Note that

$$\omega_N^{-2j} = (e^{2\pi i/N})^{-2j} = e^{-2\pi i j/(N/2)} = \omega_{N/2}^{-j}.$$

Hence $\omega_N^{-2ji} = \omega_{N/2}^{-ji}$ and therefore

$$\tilde{f}_j = \sum_{i=0}^{\frac{N}{2}-1} e_i \omega_{N/2}^{-ji} + \omega_N^{-j} \sum_{i=0}^{\frac{N}{2}-1} o_i \omega_{N/2}^{-ji}. \quad (\text{III.I5})$$

Define the length- $N/2$ DFTs

$$\tilde{e}_j := \sum_{i=0}^{\frac{N}{2}-1} e_i \omega_{N/2}^{-ji}, \quad \tilde{o}_j := \sum_{i=0}^{\frac{N}{2}-1} o_i \omega_{N/2}^{-ji}, \quad j = 0, \dots, \frac{N}{2} - 1.$$

Then, for $j = 0, 1, \dots, \frac{N}{2} - 1$,

$$\boxed{\tilde{f}_j = \tilde{e}_j + \omega_N^{-j} \tilde{o}_j} \quad (\text{III.I6})$$

THE SECOND HALF: $\tilde{f}_{j+N/2}$

Now compute for $j = \frac{N}{2} - 1, \dots, N$:

$$\tilde{f}_{j+\frac{N}{2}} = \tilde{e}_{j+\frac{N}{2}} + \omega_N^{-(j+\frac{N}{2})} \tilde{o}_{j+\frac{N}{2}}. \quad (\text{III.I7})$$

Because \tilde{e}_j and \tilde{o}_j are DFTs of length $N/2$, they are periodic with period $N/2$:

$$\tilde{e}_{j+\frac{N}{2}} = \tilde{e}_j, \quad \tilde{o}_{j+\frac{N}{2}} = \tilde{o}_j.$$

Also,

$$\omega_N^{-(j+\frac{N}{2})} = \omega_N^{-j} \omega_N^{-\frac{N}{2}}, \quad \omega_N^{-\frac{N}{2}} = e^{-2\pi i \frac{N/2}{N}} = e^{-\pi i} = -1.$$

So

$$\omega_N^{-(j+\frac{N}{2})} = -\omega_N^{-j},$$

and therefore

$$\boxed{\tilde{f}_{j+\frac{N}{2}} = \tilde{e}_j - \omega_N^{-j} \tilde{o}_j} \quad (\text{III.18})$$

COST OF ONE SPLIT (VS. FULL DFT)

The full DFT is $\mathcal{O}(N^2)$. After one split, we compute two DFTs of size $N/2$:

$$2 \left(\frac{N}{2} \right)^2 = \frac{N^2}{2}.$$

Then we combine them using

$$\tilde{f}_j = \tilde{e}_j + \omega_N^{-j} \tilde{o}_j, \quad \tilde{f}_{j+\frac{N}{2}} = \tilde{e}_j - \omega_N^{-j} \tilde{o}_j,$$

which requires multiplying by ω_N^{-j} for $j = 0, \dots, \frac{N}{2} - 1$, i.e. about $\frac{N}{2}$ extra multiplications.

So the (very rough) multiplication count becomes

$$\frac{N^2}{2} + \frac{N}{2},$$

which is about $\sim 50\%$ fewer multiplications than the original N^2 (for large N).

RECURSIVE IDEA AND THE $N \log N$ BOUND

Instead of doing one split, recursively split each DFT of size $N/2$ into two DFTs of size $N/4$, and so on, until $N = 2$.

Let $N = 2^n$ and define T_n as the number of complex multiplications required for an input of size 2^n . At each stage:

- we compute two smaller FFTs: cost $2T_{n-1}$,
- we multiply by twiddle factors ω_N^{-j} for $j = 0, \dots, 2^{n-1} - 1$: cost 2^{n-1} .

So the recurrence is

$$\boxed{T_n = 2T_{n-1} + 2^{n-1}} \quad (\text{III.19})$$

A convenient bound/solution is:

$$T_n \leq n 2^{n-1}.$$

Since $N = 2^n$, this is

$$T_n = \mathcal{O}(n2^n) = \mathcal{O}(N \log N).$$

So the running time is bounded by $N \log N$.

APPLICATION OF FFT: FAST POLYNOMIAL MULTIPLICATION

Let

$$f(x) = a_0 + a_1x + \dots + a_{N-1}x^{N-1}, \quad g(x) = b_0 + b_1x + \dots + b_{N-1}x^{N-1}.$$

Then

$$f(x)g(x) = \sum_{i=0}^{N-1} \sum_{j=0}^{N-1} a_i b_j x^{i+j} = \sum_{k=0}^{2(N-1)} c_k x^k, \quad (\text{III.20})$$

where the coefficients are the convolution

$$c_k = \sum_{i=0}^k a_i b_{k-i}. \quad (\text{III.21})$$

Directly computing all c_k costs $\mathcal{O}(N^2)$.

ALTERNATIVE VIA FFT (CONVOLUTION THEOREM)

$$\text{DFT}(f * g) = \text{DFT}(f) \cdot \text{DFT}(g) \quad (\text{pointwise product}).$$

Practical steps:

1. Zero-pad the coefficient vectors so both have the same length (typically at least $2N$).

2. Compute FFTs:

$$\tilde{a} = \text{FFT}(a), \quad \tilde{b} = \text{FFT}(b) \quad \Rightarrow \quad \mathcal{O}(N \log N).$$

3. Multiply pointwise:

$$\tilde{c}_u = \tilde{a}_u \tilde{b}_u \quad \Rightarrow \quad \mathcal{O}(N).$$

4. Inverse FFT to get c :

$$c = \text{IFFT}(\tilde{c}) \quad \Rightarrow \quad \mathcal{O}(N \log N).$$

QUANTUM FOURIER TRANSFORM

Now, we start exploring the quantum Fourier transform (QFT). In this case, let's assume a classical DFT for $N = 2$ and see how it is related to Hadamard:

Let

$$a = \begin{pmatrix} a_0 \\ a_1 \end{pmatrix}, \quad \tilde{a} = \begin{pmatrix} \tilde{a}_0 \\ \tilde{a}_1 \end{pmatrix}, \quad (N = 2).$$

The (classical) DFT is

$$\tilde{a}_k = \sum_{n=0}^{N-1} a_n \omega_N^{kn}, \quad \omega_N = e^{-2\pi i/N}.$$

For $N = 2$,

$$\omega_2 = e^{-2\pi i/2} = e^{-\pi i} = -1.$$

Hence

$$k = 0 : \quad \tilde{a}_0 = a_0 \omega_2^0 + a_1 \omega_2^0 = a_0 + a_1,$$

$$k = 1 : \quad \tilde{a}_1 = a_0 \omega_2^0 + a_1 \omega_2^1 = a_0 - a_1.$$

As a matrix multiplication,

$$\tilde{a} = \begin{pmatrix} 1 & 1 \\ 1 & -1 \end{pmatrix} \begin{pmatrix} a_0 \\ a_1 \end{pmatrix}.$$

This looks like the Hadamard transform:

$$H = \frac{1}{\sqrt{2}} \begin{pmatrix} 1 & 1 \\ 1 & -1 \end{pmatrix} \quad (N = 2).$$

So if we start with the state $a_0 |0\rangle + a_1 |1\rangle$, then applying H gives

$$H(a_0 |0\rangle + a_1 |1\rangle) = \frac{1}{\sqrt{2}}(a_0 + a_1) |0\rangle + \frac{1}{\sqrt{2}}(a_0 - a_1) |1\rangle = \tilde{a}_0 |0\rangle + \tilde{a}_1 |1\rangle,$$

where (with the QFT normalization)

$$\tilde{a}_0 = \frac{a_0 + a_1}{\sqrt{2}}, \quad \tilde{a}_1 = \frac{a_0 - a_1}{\sqrt{2}}.$$

DEFINITION OF QFT

Write a state $\sum_{x=0}^{N-1} a_x |x\rangle$. The QFT produces amplitudes

$$\tilde{a}_x = \frac{1}{\sqrt{N}} \sum_{y=0}^{N-1} \omega_N^{-xy} a_y,$$

So the QFT is:

$$|x\rangle \mapsto \frac{1}{\sqrt{N}} \sum_{y=0}^{N-1} \omega_N^{-xy} |y\rangle.$$

Thus the QFT operator can be written as

$$U_{\text{QFT}} = \frac{1}{\sqrt{N}} \sum_{x=0}^{N-1} \sum_{y=0}^{N-1} \omega_N^{-yx} |y\rangle \langle x|.$$

UNITARITY CHECK (SKETCH)

Compute:

$$\begin{aligned}
 U_{\text{QFT}} U_{\text{QFT}}^\dagger &= \frac{1}{N} \sum_{x,y} \sum_{x',y'} \omega_N^{-yx} \omega_N^{y'x'} |y\rangle \langle x| x' \langle y'| \\
 &= \frac{1}{N} \sum_x \sum_{y,y'} \omega_N^{-yx} \omega_N^{y'x} |y\rangle \langle y'| \\
 &= \frac{1}{N} \sum_{y,y'} \left(\sum_{x=0}^{N-1} \omega_N^{x(y'-y)} \right) |y\rangle \langle y'|.
 \end{aligned}$$

Using the standard identity

$$\sum_{x=0}^{N-1} \omega_N^{x(y'-y)} = N \delta_{y,y'},$$

we get

$$U_{\text{QFT}} U_{\text{QFT}}^\dagger = \sum_{y=0}^{N-1} |y\rangle \langle y| = I.$$

DEEPER STRUCTURE FOR $N = 2^n$

Assume $N = 2^n$ and $\omega_N = e^{-2\pi i/N}$. Then

$$|x\rangle \mapsto \frac{1}{\sqrt{2^n}} \sum_{y=0}^{2^n-1} \omega_N^{-xy} |y\rangle, \quad x \in \{0, 1, \dots, 2^n - 1\}.$$

Write y in binary:

$$y \in \{0, 1, \dots, 2^n - 1\}, \quad y = \sum_{k=1}^n y_k 2^{n-k}, \quad y_k \in \{0, 1\}.$$

Then

$$|x\rangle \mapsto \frac{1}{\sqrt{2^n}} \sum_{y_1, \dots, y_n \in \{0,1\}} \omega_N^{-x(\sum_{k=1}^n y_k 2^{n-k})} |y_1 \cdots y_n\rangle.$$

Because exponents add, we can factor:

$$\omega_N^{-x(\sum_{k=1}^n y_k 2^{n-k})} = \prod_{k=1}^n \omega_N^{-x 2^{n-k} y_k}.$$

So the transform becomes

$$|x\rangle \mapsto \frac{1}{\sqrt{2^n}} \sum_{y_1, \dots, y_n \in \{0,1\}} \left(\prod_{k=1}^n \omega_N^{-x 2^{n-k} y_k} \right) |y_1 \cdots y_n\rangle.$$

For each k , since $y_k \in \{0, 1\}$,

$$\sum_{y_k \in \{0,1\}} \omega_N^{-x 2^{n-k} y_k} |y_k\rangle = |0\rangle + \omega_N^{-x 2^{n-k}} |1\rangle.$$

Therefore the whole QFT output factors as a tensor product:

$$|x\rangle \mapsto \frac{1}{\sqrt{2^n}} \bigotimes_{k=1}^n \left(|0\rangle + \omega_N^{-x 2^{n-k}} |1\rangle \right).$$

WRITING PHASES USING THE BITS OF x (BINARY FRACTION)

Write x in binary:

$$|x\rangle = |x_1 x_2 \cdots x_n\rangle, \quad x_j \in \{0, 1\},$$

where x_1 is the most significant bit (MSB) and x_n is the least significant bit (LSB), so

$$x = x_1 2^{n-1} + x_2 2^{n-2} + \cdots + x_n 2^0.$$

One often rewrites the QFT result in the “gate-by-gate” form:

$$|x\rangle \mapsto \bigotimes_{k=1}^n \left(\frac{1}{\sqrt{2}} \left(|0\rangle + e^{2\pi i (0.x_k x_{k+1} \cdots x_n)} |1\rangle \right) \right)$$

where $0.x_k x_{k+1} \cdots x_n$ denotes a *binary fraction*.

BINARY FRACTION EXAMPLE

For example, if $|x\rangle = |101\rangle$ then $x_1 = 1$, $x_2 = 0$, $x_3 = 1$ and

$$0.x_1x_2x_3 = 0.101_2 = \frac{1}{2} + \frac{0}{4} + \frac{1}{8}.$$

The second qubit phase involves

$$0.x_2x_3 = 0.01_2 = \frac{0}{2} + \frac{1}{4} = \frac{1}{4}.$$

The third qubit phase involves

$$0.x_3 = 0.1_2 = \frac{1}{2}.$$

So each output qubit “sees” fewer and fewer of the input bits.

CIRCUIT EXAMPLE: $n = 3$

Let

$$|x_1x_2x_3\rangle = |101\rangle, \quad (x_1 = 1, x_2 = 0, x_3 = 1).$$

III.O.I HADAMARD ON A SINGLE QUBIT.

If Hadamard acts on a qubit $|b\rangle$ with $b \in \{0, 1\}$, then

$$H|b\rangle = \frac{1}{\sqrt{2}} (|0\rangle + (-1)^b |1\rangle).$$

STEP I: ACT ON QUBIT I

Apply H to the first qubit ($x_1 = 1$):

$$H|1\rangle = \frac{1}{\sqrt{2}} (|0\rangle - |1\rangle).$$

(Equivalently, since $0.x_1 = 0.1_2 = \frac{1}{2}$, we have $e^{2\pi i(0.x_1)} = e^{2\pi i(1/2)} = e^{\pi i} = -1$.)

CONTROLLED PHASE ROTATIONS ON QUBIT 1

The controlled- R_k phase gates (acting on the target when the control is $|1\rangle$) are:

$$R_1 = \begin{pmatrix} 1 & 0 \\ 0 & e^{2\pi i/2} \end{pmatrix}, \quad R_2 = \begin{pmatrix} 1 & 0 \\ 0 & e^{2\pi i/4} \end{pmatrix}, \quad R_3 = \begin{pmatrix} 1 & 0 \\ 0 & e^{2\pi i/8} \end{pmatrix}.$$

For $|x\rangle = |1, 0, 1\rangle$:

$x_2 = 0 \Rightarrow$ control is 0 \Rightarrow no action (on qubit 1),

$x_3 = 1 \Rightarrow$ control is 1 \Rightarrow apply R_3 to qubit 1.

Since

$$e^{2\pi i/8} = e^{i\pi/4},$$

the first-qubit state updates from

$$\frac{1}{\sqrt{2}}(|0\rangle - |1\rangle) \quad \mapsto \quad \frac{1}{\sqrt{2}}(|0\rangle - e^{i\pi/4}|1\rangle).$$

STEP 2: MOVE TO QUBIT 2

The second qubit is initially $|0\rangle$, so after Hadamard:

$$H|0\rangle = \frac{1}{\sqrt{2}}(|0\rangle + |1\rangle).$$

Because $x_3 = 1$, the controlled- R_2 acting on qubit 2 is activated, so

$$|1\rangle \mapsto e^{2\pi i/4}|1\rangle = e^{i\pi/2}|1\rangle = i|1\rangle.$$

Hence the second-qubit state becomes

$$\frac{1}{\sqrt{2}}(|0\rangle + i|1\rangle).$$

STEP 3: MOVE TO QUBIT 3

Now go to the third qubit. Since $x_3 = 1$,

$$H |1\rangle = \frac{1}{\sqrt{2}} (|0\rangle - |1\rangle).$$

There are no controlled- R_k gates from qubits below qubit 3, so no further controlled phase gate is applied to qubit 3.